\documentclass[aspectratio=1610,8pt]{beamer}

% Standard packages

\usepackage[english]{babel}
%\usepackage[latin1]{inputenc}
%\usepackage{times}
%\usepackage[T1]{fontenc}
\usepackage{fontspec}
\usepackage[]{unicode-math}
\setmathfont{Inconsolata}
\setsansfont{Roboto}

% Setup TikZ

\usepackage{tikz}
\usetikzlibrary{arrows}
\tikzstyle{block}=[draw opacity=0.7,line width=1.4cm]


% Author, Title, etc.

\title{Miscellaneous Problems on A.P., G.P. and H.P.\\Problems 121-130}

\author[Shiv Shankar Dayal]{Shiv Shankar Dayal}

% The main document

\begin{document}
\begin{frame}
  \titlepage
\end{frame}
\begin{frame}{Problem 121}
  \textbf{121.} The sum of first ten terms of an A.P. is equal to $155,$ and the sum of first two terms of a G.P. is $9.$ Find
  these progressions if the first term of the A.P. euqals the common ratio of the G.P. and the first term of G.P. equals the common
  difference of A.P.
\end{frame}
\begin{frame}{Solution of Problem 121}
  \textbf{Solution:} Let $a$ be the first term and $d$ be the common difference of A.P. and thus $d$ will be the first term and $a$
  be the common ratio of the G.P. Given,
  $$155 = \frac{10}{2}[2a + (10 - 1)d] \Rightarrow 2a + 9d = 31$$
  $$d + ad = 9$$
  $$\Rightarrow a = \frac{25}{2}, 2 \Rightarrow d = \frac{2}{3}, 3$$
  Thus, A.P. is $2, 5, 8, \ldots$ or $\frac{25}{2}, \frac{79}{6}, \frac{83}{6}, \ldots$ and the G.P. is $3, 6, 12, \ldots$ or
  $\frac{2}{3}, \frac{25}{3}, \frac{625}{6}, \ldots$
\end{frame}
\begin{frame}{Problem 122}
  \textbf{122.} If $a, b, c$ be in H.P., prove that $\left(\frac{1}{a} + \frac{1}{b} - \frac{1}{c}\right)\left(\frac{1}{b} +
  \frac{1}{c} - \frac{1}{a}\right) = \frac{4}{ac} - \frac{3}{b^2}$
\end{frame}
\begin{frame}{Solution of Problem 122}
  \textbf{Solution:} Since $a, b, c$ are in H.P. therefore $\frac{1}{a}, \frac{1}{b}, \frac{1}{c}$ are in A.P.
  \linebreak\linebreak
  $\Rightarrow \frac{2}{b} = \frac{1}{a} + \frac{1}{c} \Rightarrow b = \frac{2ac}{a + c} \Rightarrow \frac{3}{b} - \frac{2}{c} =
  \frac{1}{a} + \frac{1}{b} - \frac{1}{c} \text{~and~}\frac{3}{b} - \frac{2}{a} = \frac{1}{b} + \frac{1}{c} - \frac{1}{a}$
  $$\left(\frac{1}{a} + \frac{1}{b} - \frac{1}{c}\right)\left(\frac{1}{b} + \frac{1}{c} - \frac{1}{a}\right) = \left(\frac{3}{b} -
  \frac{2}{c}\right)\left(\frac{3}{b} - \frac{2}{a}\right)$$
  $$= \frac{9ac - 6ab - 6bc + 4b^2}{acb^2} = \frac{4}{ac} + \frac{9}{b^2} - \frac{6b(a + c)}{acb^2}$$
  $$= \frac{4}{ac} + \frac{9}{b^2} - \frac{6b}{acb^2}.\frac{2}{b}$$
  $$= \frac{4}{ac} - \frac{3}{b^2}$$
\end{frame}
\end{document}
