\documentclass[aspectratio=1610,8pt]{beamer}

% Standard packages

\usepackage[english]{babel}
%\usepackage[latin1]{inputenc}
%\usepackage{times}
%\usepackage[T1]{fontenc}


% Setup TikZ

\usepackage{tikz}
\usetikzlibrary{arrows}
\tikzstyle{block}=[draw opacity=0.7,line width=1.4cm]


% Author, Title, etc.

\title{Geometric Progression\\Problems 41-50}

\author[Shiv Shankar Dayal]{Shiv Shankar Dayal}

% The main document

\begin{document}
\begin{frame}
       \titlepage
\end{frame}
\begin{frame}{Problem 41}
  \textbf{41.} Find $1 + \frac{1}{2} + \frac{1}{4} + \frac{1}{8} + \ldots$ to $n$ terms.
\end{frame}
\begin{frame}{Solution to Problem 41}
  \textbf{Solution:} Here given sequence is a G.P. with $a = 1, r = \frac{1}{2}, n = n$

  $$S_n = \frac{a(1- r^n)}{1 - r} = \frac{1\left(1 - \frac{1}{2^n}\right)}{1 - \frac{1}{2}} = 2\left(1 - \frac{1}{2^n}\right)$$
\end{frame}
\begin{frame}{Problem 42}
    \textbf{42.} Find $1 + 2 + 4 + 8 + \ldots$ to $12$ terms.
\end{frame}
\begin{frame}{Solution to Problem 42}
  \textbf{Solution:} Here given sequence is a G.P. with $a = 1, r = 2, n = 12$

  $$S_{12} = \frac{a(r^n - 1)}{r - 1} = \frac{1(2^{12} - 1)}{2 - 1} = 4095$$
\end{frame}
\begin{frame}{Problem 43}
  \textbf{43.} Find $1 - 3 + 9 - 27 + \ldots$ to $9$ terms.
\end{frame}
\begin{frame}{Solution to Problem 43}
  \textbf{solution:} Here given sequence is a G.P. with $a = 1, r= -3, n = 9$

  $$S_9 = \frac{a(r^n - 1)}{r - 1} = \frac{1(-3^9 - 1))}{-3 - 1} = 4921$$
\end{frame}
\begin{frame}{Problem 44}
    \textbf{44.} Find $1 + \frac{1}{3} + \frac{1}{9} + \frac{1}{27} \ldots$ to $n$ terms.
\end{frame}
\begin{frame}{Solution to Problem 44}
  \textbf{Solution:} Here given seuqence is a G.P. with $a = 1, r = \frac{1}{3}, n =  n$

  $$S_n = \frac{a(1 - r^n)}{1 - r} = \frac{1\left(1 - \frac{1}{3^n}\right)}{1 - \frac{1}{3}} = \frac{3}{2}\left(1 - \frac{1}{3^n}\right)$$
\end{frame}
\begin{frame}{Problem 45}
  \textbf{45.} Find the sum of $n$ terms of the series $(a + b) + (a^2 + 2b) + (a^3 + 3b) + \ldots$ to $n$ terms.
\end{frame}
\begin{frame}{Solution of Problem 45}
  \textbf{Solution:} $(a + b) + (a^2 + 2b) + (a^3 + 3b) + \ldots$ to $n$ terms

  $$=(a + a^2 + a^3 + \ldots)~\text{to}~n~\text{terms} + b(1 + 2 + 3 + \ldots)~\text{to}~n~\text{terms}$$
  $$= \frac{a(1 - a^n)}{1 - a} + b.\frac{n(n + 1)}{2}$$
\end{frame}
\begin{frame}{Problem 46}
  \textbf{46.} A man agrees to work at the rate of one dollar the first day, two dollars the second day, four dollars the third
  day, eight dollars the fourth day and so on. How much would he get at the end of $120$ days.
\end{frame}
\begin{frame}{Solution of Problem 46}
  \textbf{Solution:} Total amount rececived at the end of $120$ days

  $$= 1 + 2 + 4 + 8~\text{to}~120~\text{terms}$$
  $$= \frac{1.(2^{120} - 1)}{2 - 1} = 2^{120} - 1$$
  $$= 1329227995784915872903807060280344575$$
\end{frame}
\begin{frame}{Problem 47}
  \textbf{47.} Find the sum to $n$ terms of the series $8 + 88 + 888 + \ldots$
\end{frame}
\begin{frame}{Solution of Problem 47}
  \textbf{Solution:} Let $S_n = 8 + 88 + 888 +  \ldots$ to $n$ terms
  $$= 8[1 + 11 + 111 + \ldots]$$
  $$ = \frac{8}{9}[9 + 99 + 999 + \ldots]$$
  $$= \frac{8}{9}[(10 - 1) + (100 - 1) + (1000 - 1) + \ldots]$$
  $$= \frac{8}{9}[(10 + 100 + 1000 + \ldots) - (1 + 1 + 1 + \ldots)]$$
  $$= \frac{8}{9}\left[10\left(\frac{10^n - 1}{10 - 1}\right) - n\right]$$
  $$= \frac{8}{81}(10^{n + 1} - 10 - 9n)$$
\end{frame}
\begin{frame}{Problem 48}
  \textbf{48.} Find the sum to $n$ terms of the series $6 + 66 + 666 + \ldots$
\end{frame}
\begin{frame}{Solution of Problem 48}
  \textbf{Solution:} Let $S_n = 6 + 66 + 666 +  \ldots$ to $n$ terms
  $$= 6[1 + 11 + 111 + \ldots]$$
  $$ = \frac{6}{9}[9 + 99 + 999 + \ldots]$$
  $$= \frac{2}{3}[(10 - 1) + (100 - 1) + (1000 - 1) + \ldots]$$
  $$= \frac{2}{3}[(10 + 100 + 1000 + \ldots) - (1 + 1 + 1 + \ldots)]$$
  $$= \frac{2}{3}\left[10\left(\frac{10^n - 1}{10 - 1}\right) - n\right]$$
  $$= \frac{2}{27}(10^{n + 1} - 10 - 9n)$$
\end{frame}
\begin{frame}{Problem 49}
  \textbf{49.} Find the sum to $n$ terms of the series $4 + 44 + 444 + \ldots$
\end{frame}
\begin{frame}{Solution of Problem 49}
  \textbf{Solution:} Let $S_n = 4 + 44 + 444 +  \ldots$ to $n$ terms
  $$= 4[1 + 11 + 111 + \ldots]$$
  $$ = \frac{4}{9}[9 + 99 + 999 + \ldots]$$
  $$= \frac{4}{9}[(10 - 1) + (100 - 1) + (1000 - 1) + \ldots]$$
  $$= \frac{4}{9}[(10 + 100 + 1000 + \ldots) - (1 + 1 + 1 + \ldots)]$$
  $$= \frac{4}{9}\left[10\left(\frac{10^n - 1}{10 - 1}\right) - n\right]$$
  $$= \frac{4}{81}(10^{n + 1} - 10 - 9n)$$
\end{frame}
\begin{frame}{Problem 50}
  \textbf{50.} Find the sum to $n$ terms of the series $.5 + .55 + .555 + \ldots$
\end{frame}
\begin{frame}{Solution of Problem 50}
  \textbf{Solution:} Let $S_n = .5 + .55 + .555 +  \ldots$ to $n$ terms
  $$= 5[.1 + .11 + .111 + \ldots]$$
  $$ = \frac{5}{9}[.9 + .99 + .999 + \ldots]$$
  $$= \frac{5}{9}[(1 - .1) + (1 - .01) + (1 - .001) + \ldots]$$
  $$= \frac{5}{9}[(1 + 1 + 1 + \ldots) - (.1 + .01 + .001)]$$
  $$= \frac{5}{9}\left[n - \frac{1}{10}\frac{\frac{1}{1 - 10^n}}{1 - \frac{1}{9}}\right]$$
\end{frame}
\end{document}
