\documentclass[aspectratio=1610,8pt]{beamer}

% Standard packages

\usepackage[english]{babel}
%\usepackage[latin1]{inputenc}
%\usepackage{times}
%\usepackage[T1]{fontenc}
\usepackage{fontspec}
\usepackage[]{unicode-math}
\setmathfont{Inconsolata}
\setsansfont{Roboto}
% Setup TikZ

\usepackage{tikz}
\usetikzlibrary{arrows}
\tikzstyle{block}=[draw opacity=0.7,line width=1.4cm]

\newcounter{counter}

% Author, Title, etc.
\title{Logarithm Problem 21-30}

\author[Shiv Shankar Dayal]{Shiv Shankar Dayal}

% The main document

\begin{document}
\begin{frame}
  \titlepage
\end{frame}
\begin{frame}{Problem 21}
  \textbf{21.} Simplify $\frac{\log_911}{\log_513}\div\frac{\log_311}{\log_{\sqrt{5}}13}$
\end{frame}
\begin{frame}{Solution of Problem 21}
  \textbf{Solution:} Given $$\frac{\log_911}{\log_513}\div\frac{\log_311}{\log_{\sqrt{5}}13}$$
  $$= \frac{\log_{3^2}11}{\log_513}.\frac{\log_{5^{\frac{1}{2}}}13}{\log_311}$$
  $$= \frac{\frac{1}{2}\log_311}{\log_513}.\frac{2\log_513}{\log_311} = 1$$
\end{frame}
\begin{frame}{Problem 22}
  \textbf{22.} Simplify $3^{\sqrt{\log_32}} - 2^{\sqrt{\log_23}}$
\end{frame}
\begin{frame}{Solution of Problem 22}
  \textbf{Solution:} Taking $\log$ with base $10,$ we get
  $$= \sqrt{\log_32}\log 3 - \sqrt{\log_23}\log 2$$
  $$= \sqrt{\frac{\log2}{\log3}(\log 3)^2} - \sqrt{\frac{\log3}{\log2}(\log2)^2}$$
  $$=\sqrt{\log2\log3} - \sqrt{\log3\log2} = 0$$
\end{frame}
\begin{frame}{Problem 23}
  \textbf{23.} Find the least integer $n$ such that $7^n > 10^5,$ given that $\log_{10}343 = 2.5353$
\end{frame}
\begin{frame}{Solution of Problem 23}
  \textbf{Solution:} $$\log_{10}343 = 2.5353 \Rightarrow \log_{10}7^3 = 2.5353 \Rightarrow \log_{10}7 = 0.8451$$
  $$7^n > 10^5 \Rightarrow n\log_{10}7 > 5\Rightarrow n > \frac{5}{0.8451}$$
  Thus, least value of such integer is $6.$
\end{frame}
\begin{frame}{Problem 24}
  \textbf{24.} If $a,b,c$ are in G.P. then prove that $\log_ax, \log_bx,
  \log_cx$ are in H.P.
\end{frame}
\begin{frame}{Solution of Problem 24}
  \textbf{Solution:} Since $a,b,c$ are in G.P. therefore we can write $b^ = ac$
  \linebreak\linebreak
  Taking $log,$ on both sides, we get $2\log b = \log a + \log c.$
  Thus, $\log a, \log b, \log c$ are in A.P.
  \linebreak\linebreak
  $\therefore \frac{1}{\log a}, \frac{1}{\log b}, \frac{1}{\log c}$ are in H.P.
  \linebreak\linebreak
  $\therefore~ \frac{\log x}{\log a}, \frac{\log x}{\log b}, \frac{\log x}{\log c}$ are in H.P.
  \linebreak\linebreak
  $\therefore~\log_xa, \log_xb, \log_xc$ are in H.P.
\end{frame}
\begin{frame}{Problem 25}
  \textbf{25.} Prove that $\log \sin8x = 3\log2 + \log\sin x + \log\cos x + \log\cos2x + \log\cos4x$
\end{frame}
\begin{frame}{Solution of Problem 25}
  \textbf{Solution:} $$L.H.S. - \log\sin8x = \log2\sin4x\cos4x$$
  $$= \log 2 + \log\sin4x + \log\cos4x$$
  $$=\log2 + \log2\sin2x\cos2x + \log\cos4x$$
  $$= 2\log2 + \log\sin2x + \log\cos2x + \log\cos4x$$
  $$= 2\log 2 + \log2\sin x\cos x + \log\cos2x + \log\cos4x$$
  $$= 4\log2 + \log \sin x + \log\cos x + \log\cos2x + \log\cos4x = R.H.S.$$
\end{frame}
\begin{frame}{Problem 26}
  \textbf{26.} If $x=\log_{2a}a, y =\log_{3a}2a$ and $z = \log_{4a}3a,$ then prove that $xyz + 1 = 2yz$
\end{frame}
\begin{frame}{Solution of Problem 26}
  \textbf{Solution:} We have to prove that $xyz +1 = 2yx$
  \linebreak\linebreak
  Dividing both sides with $yz,$ we get $x + \frac{1}{yz} = 2$
  $$L.H.S. = \log_{2a}a + \frac{1}{\log_{3a}2a\log_{4a}3a}$$
  $$= \frac{\log a}{\log 2a} + \frac{\log 3a\log 4a}{\log 2a\log 3a}$$
  $$= \frac{\log a}{\log 2a} + \frac{\log 4a}{\log 2a}$$
  $$= \frac{\log a + \log 4a}{\log 2a} = \frac{\log(2a)^2}{\log 2a} = 2 = R.H.S.$$
\end{frame}
\begin{frame}{Problem 27}
  \textbf{27.} If $a$ and $b$ are lengths of the sides and $c$ be the length of hypotenuse of a right angle triangle and $c - b\neq
  1$ and $c + b\neq 1,$ prove that $\log_{c + b}a + \log_{c - b}a = 2\log_{c+b}a\log_{c - b}a$
\end{frame}
\begin{frame}{Solution of Problem 27}
  \textbf{Solution:} We have to prove that $\log_{c + b}a + \log_{c - b}a = 2\log_{c+b}a\log_{c - b}a$
  \linebreak\linebreak
  Dividing both side by $\log_{c + b}a\log_{c - b}a,$ we get
  $$L.H.S. = \frac{1}{\log_{c - b}a} + \frac{1}{\log_{c + b}a} = 2$$
  $$\log_a(c - b) + \log_a(c + b) = 2$$
  $$\log_a(c^2 - b^2) = a \Rightarrow c^2 - b^2 = a^2$$
  $$\Rightarrow c^2 = a^2 + b^2$$
  which is true for the given right angle triangle.
\end{frame}
\begin{frame}{Problem 28}
  \textbf{28.} If $\frac{\log z}{y - z} = \frac{\log y}{z - x} = \frac{\log z}{x - y},$ then prove that $x^xy^yz^x = 1$
\end{frame}
\begin{frame}{Solution of Problem 28}
  \textbf{Solution:} Let $\frac{\log z}{y - z} = \frac{\log y}{z - x} = \frac{\log z}{x - y} = k$
  $$\Rightarrow \log x = k(y - z), \log y = k(z - x), \log z = k(x - y)$$
  We have to prove that $x^xy^yz^z = 1$
  Taking $\log$ of both sides, we get
  $$x\log x + y\log y + z\log z = 0$$
  $$kx(y - z) + ky(z - x) + kz(x - y) = 0$$
  $$0 = 0$$
\end{frame}
\begin{frame}{Problem 29}
  \textbf{29.} If $\frac{yz\log(yz)}{y + z} = \frac{zx\log(zx)}{z + x} = \frac{xy\log(xy)}{x + y},$ then prove that $x^x = y^y = z^z$
\end{frame}
\begin{frame}{Solution of Problem 29}
  \textbf{Solution:} Given, $\frac{yz\log(yz)}{y + z} = \frac{zx\log(zx)}{z + x} = \frac{xy\log(xy)}{x + y}$
  \linebreak\linebreak
  Dividing each term by $xyz,$ we get
  $$\frac{\log y + \log z}{xy + zx} = \frac{\log z + \log x}{yz + xy} = \frac{\log x + \log y}{zx + yz} = k(\text{let})$$
  $$\log y + \log z = k(xy + zx), \log z + \log x = k(yz + zx), \log x + \log y = k(zx + yz)$$
  $$2(\log x + \log y + \log z) = 2k(xy + yz + zx)$$
  $$\therefore ~\log x = kyz \Rightarrow x\log x = kxyz$$
  $$\text{Similarly,} \log y = kzx \Rightarrow y\log y = kxyz$$
  $$\log z = kxy \Rightarrow z\log z = kxyz$$
  $$\therefore x\log x = y\log y = z\log z$$
  $$\therefore x^x = y^y = z^z$$
\end{frame}
\begin{frame}{Problem 30}
  \textbf{30.} Prove that $(yz)^{\log y - \log z}zx^{\log z - \log x}(xy)^{\log x - \log y} = 1$
\end{frame}
\begin{frame}{Solution of Problem 30}
  \textbf{Solution:} Taking log of both sides, we get
  $$(\log y - \log z)(\log y + \log z) + (\log z - \log x)(\log z + \log x) + (\log x - \log y)(\log x + \log y) = 0$$
  $$(\log y)^2 - (\log z)^2 + (\log z)^2 - (\log x)^2 + (\log x)^2 - (\log y)^2 = 0$$
  $$0 = 0$$
\end{frame}
\end{document}
