\documentclass[aspectratio=1610,8pt]{beamer}

% Standard packages

\usepackage[english]{babel}
%\usepackage[latin1]{inputenc}
%\usepackage{times}
%\usepackage[T1]{fontenc}
\usepackage{fontspec}
\usepackage[]{unicode-math}
\setmathfont{Inconsolata}
\setsansfont{Roboto}
% Setup TikZ

\usepackage{tikz}
\usetikzlibrary{arrows}
\tikzstyle{block}=[draw opacity=0.7,line width=1.4cm]

\newcounter{counter}

% Author, Title, etc.
\title{Logarithm Problem 11-20}

\author[Shiv Shankar Dayal]{Shiv Shankar Dayal}

% The main document

\begin{document}
\begin{frame}
  \titlepage
\end{frame}
\begin{frame}{Problem 11}
  \textbf{11.} Prove that $\log_3\log_2\log_{\sqrt{3}}81 = 1$
\end{frame}
\begin{frame}{Solution of Problem 11}
  \textbf{Solution:} $$L.H.S. = \log_3\log_2\log_{\sqrt{3}}81 = \log_3\log_2\log_{\sqrt{3}}(\sqrt{3})^8$$
  $$= \log_3\log_28 = \log_3 3 = 1 = R.H.S.$$
\end{frame}
\begin{frame}{Problem 12}
  \textbf{12.} Prove that $\log_ax\log_by = \log_bx\log_ay$
\end{frame}
\begin{frame}{Solution of Problem 12}
  \textbf{Solution:} $$L.H.S = \log_ax\log_by = \frac{\log x}{\log a}.\frac{\log y}{\log b}$$
  $$= \frac{\log x}{\log b}.\frac{\log y}{\log a} = \log_bx\log_ay = R.H.S.$$
\end{frame}
\begin{frame}{Problem 13}
  \textbf{13.} Prove that $a^x = 10^x\log_{10}a$
\end{frame}
\begin{frame}{Solution of Problem 13}
  \textbf{Solution:} $$R.H.S. = 10^x\log_{10}a = z\text{~(say)}$$
  Taking $\log$ of both sides with base $10$
  $$\log_{10}z = x\log_{10}a = \log_{10}a^x \Rightarrow z = a^x = L.H.S.$$
\end{frame}
\begin{frame}{Problem 14}
  \textbf{14.} Prove that $\log_2\log_2\log_216 = 1$
\end{frame}
\begin{frame}{Solution of Problem 14}
  \textbf{Solution:} $$L.H.S. = \log_2\log_2\log_216 = \log_2\log_24$$
  $$=\log_22 = 1 = R.H.S.$$
\end{frame}
\begin{frame}{Problem 15}
  \textbf{15.} Prove that $\log_ax = \log_bx\log_cb\ldots\log_nm\log_an$
\end{frame}
\begin{frame}{Solution of Problem 15}
  \textbf{Solution:} $$R.H.S. = \log_bx\log_cb\ldots\log_nm\log_an$$
  $$= \frac{\log x}{\log b}.\frac{\log b}{\log c}\ldots\frac{\log m}{\log n}.\frac{\log n}{\log a}$$
  $$= \frac{\log x}{\log a} = \log_ax = L.H.S.$$
\end{frame}
\begin{frame}{Problem 16}
  \textbf{16.} If $a^2 + b^2 = 7ab,$ prove that $\log\frac{a + b}{3} = \frac{1}{2}(\log a + \log b)$
\end{frame}
\begin{frame}{Solution of Problem 16}
  \textbf{Solution:} Given, $$a^2 + b^2 = 7ab \Rightarrow a^2 + b^2 + 2ab = 9ab$$
  $$\Rightarrow \left(\frac{a + b}{3}\right)^2 = ab$$
  Taking $\log$ of both sides, we get
  $$2\log\frac{a + b}{3} = \log(ab) \Rightarrow \log\frac{a + b}{3} = \frac{1}{2}(\log a + \log b)$$
\end{frame}
\begin{frame}{Problem 17}
  \textbf{17.} Prove that $\frac{\log a(\log_ba)}{\log b(\log_ab)} = -\log_ba$
\end{frame}
\begin{frame}{Solution of Problem 17}
  \textbf{Solution:} $$L.H.S. = \frac{\log a(\log_ba)}{\log b(\log_ab)} = \frac{\log a\frac{\log a}{\log b}}{\log b\frac{\log
      a}{\log b}}$$
  $$= \frac{\log a\log a - \log a\log b}{\log b\log b - \log b\log a}$$
  $$= \frac{\log a(\log a - \log b)}{\log b(\log b - \log a)} = -\log_ba$$
\end{frame}
\begin{frame}{Problem 18}
  \textbf{18.} Prove that $\log(1 + 2 + 3) = \log 1 + \log 2 + \log 3$
\end{frame}
\begin{frame}{Solution of Problem 18}
  \textbf{Solution:} $$L.H.S. = \log(1 + 2 + 3) = \log 6 = \log (2.3) = \log 2 + \log 3$$
  $$= \log 1 + \log 2 + \log 3[\because \log 1 = 0]$$
\end{frame}
\begin{frame}{Problem 19}
  \textbf{19.} Prove that $2\log(1 + 2 + 4 + 7 + 14) = \log 1 + \log 2 + \log 4 + \log 7 + \log 14$
\end{frame}
\begin{frame}{Solution of Problem 19}
  \textbf{Solution:} $$L.H.S. = 2\log(1 + 2 + 4 + 7 + 14) = 2\log 28$$
  $$= \log 28^2 = \log 784 = \log(1.2.4.7.14) = \log 1 + \log 2 + \log 4 + \log 7 + \log 14$$
\end{frame}
\begin{frame}{Problem 20}
  \textbf{20.} Prove that $\log 2 + 16\log\frac{16}{15} + 12\log\frac{25}{24} + 3\log\frac{81}{80} = 1$
\end{frame}
\begin{frame}{Solution of Problem 20}
  \textbf{Solution:} $$L.H.S. = \log 2 + 16\log\frac{16}{15} + 12\log\frac{25}{24} + 3\log\frac{81}{80}$$
  $$= \log2 +16[\log16 - \log15] + 12[\log25 - \log24] + 7[\log81 - \log80]$$
  $$=\log2 + 16[\log2^4 - \log3*5] + 12[\log5^2 - \log2^3*3] + 7[\log3^4 - \log2^4*5]$$
  $$=\log2 + 16[4\log2 -\log3 -\log5]+12[2\log5 - 3\log2 -\log3] + 7[4\log3 - 4\log2 - \log 5]$$
  $$= \log2[1 + 64 - 36 - 28] + \log 3[28 - 16 - 12] + \log5[24 - 7 - 16]$$
  $$=\log 2 + \log5 = \log 10 = 1[\text{~default base is~} 10 \text{~for common logarithms}]$$
\end{frame}
\end{document}
